Fix inferencer and remove all cheats in inferComplete

compiler/inference/inferScript.sml
@@ -600,7 +600,8 @@ val check_specs_def = Define `
 (check_specs mn tenvT decls tenvT' cenv env (Sval x t::specs) =
   do fvs <- t_to_freevars t;
      fvs' <- return (nub fvs);
-     check_specs mn tenvT decls tenvT' cenv ((x, (LENGTH fvs', infer_type_subst (ZIP (fvs', MAP Infer_Tvar_db (COUNT_LIST (LENGTH fvs')))) t)) :: env) specs
+     () <- guard (check_type_names tenvT t) "Bad type annotation";
+     check_specs mn tenvT decls tenvT' cenv ((x, (LENGTH fvs', infer_type_subst (ZIP (fvs', MAP Infer_Tvar_db (COUNT_LIST (LENGTH fvs')))) (type_name_subst tenvT t))) :: env) specs
   od) ∧
 (check_specs mn tenvT (mdecls,tdecls,edecls) tenvT' cenv env (Stype tdefs :: specs) =
   do new_tenvT <- return (FEMPTY |++ MAP (λ(tvs,tn,ctors). (tn, (tvs, Tapp (MAP Tvar tvs) (TC_name (mk_id mn tn))))) tdefs);
